erasure/theories/Extraction.v
@@ -1,5 +1,5 @@
 (* Distributed under the terms of the MIT license. *)
-From Coq Require Import FSets ExtrOcamlBasic ExtrOcamlString ExtrOcamlZInt ExtrOCamlFloats ExtrOCamlInt63.
+From Coq Require Import FSets ExtrOcamlBasic ExtrOcamlString ExtrOcamlZInt ExtrOcamlNatInt ExtrOCamlFloats ExtrOCamlInt63.
 From MetaCoq.Template Require Import utils.
 
 (** * Extraction setup for the erasure phase of template-coq.
@@ -10,7 +10,9 @@ From MetaCoq.Template Require Import utils.
 
 Extract Constant ascii_compare =>
  "fun x y -> match Char.compare x y with 0 -> Eq | x when x < 0 -> Lt | _ -> Gt".
-
+Extract Constant Ascii.compare =>
+ "fun x y -> match Char.compare x y with 0 -> Eq | x when x < 0 -> Lt | _ -> Gt".
+ 
 Extraction Blacklist Classes config uGraph Universes Ast String List Nat Int
            UnivSubst Typing Checker Retyping OrderedType Logic Common Equality Classes Numeral
            Uint63.
